src/Reflection/LinearizeInterp.v
@@ -11,14 +11,14 @@ Section language.
   Context (base_type_code : Type).
   Context (interp_base_type : base_type_code -> Type).
   Context (op : flat_type base_type_code -> flat_type base_type_code -> Type).
-  Context (interp_op : forall src dst, op src dst -> interp_flat_type_gen interp_base_type src -> interp_flat_type_gen interp_base_type dst).
+  Context (interp_op : forall src dst, op src dst -> interp_flat_type interp_base_type src -> interp_flat_type interp_base_type dst).
 
   Local Notation flat_type := (flat_type base_type_code).
   Local Notation type := (type base_type_code).
   Let Tbase := @Tbase base_type_code.
   Local Coercion Tbase : base_type_code >-> Syntax.flat_type.
   Let interp_type := interp_type interp_base_type.
-  Let interp_flat_type := interp_flat_type_gen interp_base_type.
+  Let interp_flat_type := interp_flat_type interp_base_type.
   Local Notation exprf := (@exprf base_type_code interp_base_type op).
   Local Notation expr := (@expr base_type_code interp_base_type op).
   Local Notation Expr := (@Expr base_type_code interp_base_type op).
